Started adding 'a arrays

semantics/proofs/evalPropsScript.sml
@@ -59,13 +59,13 @@ val do_app_cases = Q.store_thm ("do_app_cases",
     (op = Opderef) ∧ (vs = [Loc lnum]) ∧ (store_lookup lnum st = SOME (Refv v2)) ∧
     (v = Rval v2)) ∨
   (?i w.
-      (op = Aalloc) ∧ (vs = [Litv (IntLit i); Litv (Word8 w)]) ∧
+      (op = Aw8alloc) ∧ (vs = [Litv (IntLit i); Litv (Word8 w)]) ∧
       (((i < 0) ∧ v = Rerr (Rraise (prim_exn "Subscript")) ∧ (st = st')) ∨
        (?lnum. ~(i < 0) ∧
         (st',lnum) = store_alloc (W8array (REPLICATE (Num (ABS i)) w)) st ∧
         v = Rval (Loc lnum)))) ∨
   (?ws lnum i.
-    (op = Asub) ∧ (vs = [Loc lnum; Litv (IntLit i)]) ∧ (st = st') ∧
+    (op = Aw8sub) ∧ (vs = [Loc lnum; Litv (IntLit i)]) ∧ (st = st') ∧
     store_lookup lnum st = SOME (W8array ws) ∧ 
     (((i < 0) ∧ v = Rerr (Rraise (prim_exn "Subscript"))) ∨
      ((~(i < 0) ∧ Num (ABS i) ≥ LENGTH ws ∧
@@ -74,11 +74,11 @@ val do_app_cases = Q.store_thm ("do_app_cases",
       Num (ABS i) < LENGTH ws ∧
       (v = Rval (Litv (Word8 (EL (Num(ABS i)) ws))))))) ∨
   (?lnum ws.
-    (op = Alength) ∧ (vs = [Loc lnum]) ∧ st = st' ∧
+    (op = Aw8length) ∧ (vs = [Loc lnum]) ∧ st = st' ∧
     store_lookup lnum st = SOME (W8array ws) ∧ 
     v = Rval (Litv (IntLit (&(LENGTH ws))))) ∨
   (?ws lnum i w.
-    (op = Aupdate) ∧ (vs = [Loc lnum; Litv (IntLit i); Litv (Word8 w)]) ∧ 
+    (op = Aw8update) ∧ (vs = [Loc lnum; Litv (IntLit i); Litv (Word8 w)]) ∧ 
     store_lookup lnum st = SOME (W8array ws) ∧ 
     (((i < 0) ∧ v = Rerr (Rraise (prim_exn "Subscript")) ∧ st = st') ∨
      ((~(i < 0) ∧ Num (ABS i) ≥ LENGTH ws ∧ st = st' ∧
@@ -98,7 +98,39 @@ val do_app_cases = Q.store_thm ("do_app_cases",
        v = Rerr (Rraise (prim_exn "Subscript")))) ∨
      (~(i < 0) ∧
       Num (ABS i) < LENGTH vs' ∧
-      (v = Rval (EL (Num(ABS i)) vs'))))))`,
+      (v = Rval (EL (Num(ABS i)) vs'))))) ∨
+  (?vs'.
+    (op = Vlength) ∧ (vs = [Vectorv vs']) ∧ st = st' ∧
+    v = Rval (Litv (IntLit (&(LENGTH vs'))))) ∨
+  (?i v'.
+      (op = Aalloc) ∧ (vs = [Litv (IntLit i); v']) ∧
+      (((i < 0) ∧ v = Rerr (Rraise (prim_exn "Subscript")) ∧ (st = st')) ∨
+       (?lnum. ~(i < 0) ∧
+        (st',lnum) = store_alloc (Varray (REPLICATE (Num (ABS i)) v')) st ∧
+        v = Rval (Loc lnum)))) ∨
+  (?vs' lnum i.
+    (op = Asub) ∧ (vs = [Loc lnum; Litv (IntLit i)]) ∧ (st = st') ∧
+    store_lookup lnum st = SOME (Varray vs') ∧ 
+    (((i < 0) ∧ v = Rerr (Rraise (prim_exn "Subscript"))) ∨
+     ((~(i < 0) ∧ Num (ABS i) ≥ LENGTH vs' ∧
+       v = Rerr (Rraise (prim_exn "Subscript")))) ∨
+     (~(i < 0) ∧
+      Num (ABS i) < LENGTH vs' ∧
+      (v = Rval (EL (Num(ABS i)) vs'))))) ∨
+  (?lnum vs'.
+    (op = Alength) ∧ (vs = [Loc lnum]) ∧ st = st' ∧
+    store_lookup lnum st = SOME (Varray vs') ∧ 
+    v = Rval (Litv (IntLit (&(LENGTH vs'))))) ∨
+  (?vs' lnum i v'.
+    (op = Aupdate) ∧ (vs = [Loc lnum; Litv (IntLit i); v']) ∧ 
+    store_lookup lnum st = SOME (Varray vs') ∧ 
+    (((i < 0) ∧ v = Rerr (Rraise (prim_exn "Subscript")) ∧ st = st') ∨
+     ((~(i < 0) ∧ Num (ABS i) ≥ LENGTH vs' ∧ st = st' ∧
+       v = Rerr (Rraise (prim_exn "Subscript")))) ∨
+     (~(i < 0) ∧
+      Num (ABS i) < LENGTH vs' ∧
+      store_assign lnum (Varray (LUPDATE v' (Num (ABS i)) vs')) st = SOME st' ∧
+      v = Rval (Litv Unit)))))`,
  SIMP_TAC (srw_ss()) [do_app_def] >>
  cases_on `op` >>
  rw [] >>
@@ -106,6 +138,8 @@ val do_app_cases = Q.store_thm ("do_app_cases",
  rw [] >>
  every_case_tac >>
  rw [] >>
+ full_simp_tac (srw_ss()++ARITH_ss) [] >>
+ TRY (eq_tac >> rw [] >> NO_TAC) >>
  TRY (cases_on `do_eq v1 v2`) >>
  rw [] >>
  UNABBREV_ALL_TAC >>
@@ -324,33 +358,37 @@ val _ = export_rewrites["sv_every_def"]
 val sv_rel_def = Define`
   sv_rel R (Refv v1) (Refv v2) = R v1 v2 ∧
   sv_rel R (W8array w1) (W8array w2) = (w1 = w2) ∧
+  sv_rel R (Varray vs1) (Varray vs2) = LIST_REL R vs1 vs2 ∧
   sv_rel R _ _ = F`
 val _ = export_rewrites["sv_rel_def"]
 
 val sv_rel_refl = store_thm("sv_rel_refl",
   ``∀R x. (∀x. R x x) ⇒ sv_rel R x x``,
-  gen_tac >> Cases >> rw[sv_rel_def])
+  gen_tac >> Cases >> rw[sv_rel_def] >>
+  induct_on `l` >>
+  rw [])
 val _ = export_rewrites["sv_rel_refl"]
 
 val sv_rel_trans = store_thm("sv_rel_trans",
   ``∀R. (∀x y z. R x y ∧ R y z ⇒ R x z) ⇒ ∀x y z. sv_rel R x y ∧ sv_rel R y z ⇒ sv_rel R x z``,
-  gen_tac >> strip_tac >> Cases >> Cases >> Cases >> rw[sv_rel_def] >> metis_tac[])
+  gen_tac >> strip_tac >> Cases >> Cases >> Cases >> rw [] >> fs [sv_rel_def] >> metis_tac[miscTheory.LIST_REL_trans]);
 
 val sv_rel_cases = store_thm("sv_rel_cases",
   ``∀x y.
     sv_rel R x y ⇔
     (∃v1 v2. x = Refv v1 ∧ y = Refv v2 ∧ R v1 v2) ∨
-    (∃w. x = W8array w ∧ y = W8array w)``,
+    (∃w. x = W8array w ∧ y = W8array w) ∨
+    (?vs1 vs2. x = Varray vs1 ∧ y = Varray vs2 ∧ LIST_REL R vs1 vs2)``,
   Cases >> Cases >> simp[sv_rel_def,EQ_IMP_THM])
 
 val sv_rel_O = store_thm("sv_rel_O",
   ``∀R1 R2. sv_rel (R1 O R2) = sv_rel R1 O sv_rel R2``,
   rw[FUN_EQ_THM,sv_rel_cases,O_DEF,EQ_IMP_THM] >>
-  metis_tac[])
+  metis_tac[miscTheory.LIST_REL_O])
 
 val sv_rel_mono = store_thm("sv_rel_mono",
   ``(∀x y. P x y ⇒ Q x y) ⇒ sv_rel P x y ⇒ sv_rel Q x y``,
-  rw[sv_rel_cases])
+  rw[sv_rel_cases] >> metis_tac [LIST_REL_mono])
 
 val map_match_def = Define`
   (map_match f (Match env) = Match (f env)) ∧
